update

Licenta.dfy
@@ -1,16 +1,8 @@
-datatype Problem = Problem(numberOfObjects: int, knapsackCapacity: int, costs: seq<int>, weights: seq<int>)
-
-datatype Solution = Solution(profit: int, objects: seq<int>)
+datatype Problem = Problem(numberOfObjects: int, knapsackCapacity: int, gains: seq<int>, weights: seq<int>)
 
 predicate hasPositiveValues(input: seq<int>)
 {
     forall i :: 0 <= i < |input| ==> input[i] > 0
-}
-
-predicate isValidProblem(p: Problem)
-{
-    |p.costs| == |p.weights| == p.numberOfObjects && p.numberOfObjects > 0 && p.knapsackCapacity >= 0 && 
-          hasPositiveValues(p.costs) && hasPositiveValues(p.weights)
 }
 
 function max(p1: int, p2: int): int
@@ -18,37 +10,90 @@ function max(p1: int, p2: int): int
     if p1 > p2 then p1 else p2
 }
 
-function gain(solution: seq<int>, costs: seq<int>): int
-  requires |solution| == |costs| 
+function gain(problem: Problem, solution: seq<int>): int
+  requires isValidProblem(problem)
+  requires isValidPartialSolution(problem, solution)
 {
-  if |solution| == 0 then 0 else solution[0] * costs[0] + gain(solution[1..], costs[1..])
+  if |solution| == 0 then 0 else computeGain(problem.gains, solution, |solution| - 1)
 }
 
-predicate isValidSolution(p: Problem, solution: Solution)
+function computeGain(gains: seq<int>, solution: seq<int>, i: int) : int
+  requires 0 <= i < |solution|
+  requires 0 <= i < |gains|
 {
-  |solution.objects| == p.numberOfObjects && 
-  forall k :: 0 <= k < |solution.objects| ==> solution.objects[k] == 0 || solution.objects[k] == 1
+   if i == 0 then 0 else solution[i] * gains[i] + computeGain(gains, solution, i - 1)
 }
 
-predicate isSolution(p: Problem, solution: Solution)
+function intermediaryPartialSolution(seq1: seq<int>, seq2: seq<int>) : int
+{
+  if |seq1| == 0 || |seq2| == 0 then 0 else seq1[0] * seq2[0] + intermediaryPartialSolution(seq1[1..], seq2[1..])
+}
+
+function weight(problem: Problem, solution: seq<int>): int
+  requires isValidProblem(problem)
+  requires isValidPartialSolution(problem, solution)
+{
+  if |solution| == 0 then 0 else computeWeight(problem.weights, solution, |solution| - 1)
+}
+
+function computeWeight(weights: seq<int>, solution: seq<int>, i: int) : int
+  requires 0 <= i < |solution|
+  requires 0 <= i < |weights|
+{
+   if i == 0 then 0 else solution[i] * weights[i] + computeWeight(weights, solution, i - 1)
+}
+
+predicate isValidProblem(problem: Problem)
+{
+    |problem.gains| == |problem.weights| == problem.numberOfObjects && 
+    problem.numberOfObjects > 0 && problem.knapsackCapacity >= 0 && 
+    hasPositiveValues(problem.gains) && hasPositiveValues(problem.weights) 
+}
+
+predicate isValidSolution(problem: Problem, solution: seq<int>)
+{
+  isValidPartialSolution(problem, solution) &&
+  |solution| == problem.numberOfObjects
+}
+
+predicate isSolution(p: Problem, solution: seq<int>)
   requires isValidProblem(p)
-  requires isValidSolution(p, solution) 
 {
-  gain(solution.objects, p.costs) == solution.profit
+  isValidSolution(p, solution) &&
+  weight(p, solution) <= p.knapsackCapacity
 }
 
-predicate isPartialSolution(partialSolution: seq<int>)
+predicate isValidPartialSolution(problem: Problem, solution: seq<int>)
 {
-  forall s :: 1 <= s < |partialSolution| ==> partialSolution[s] >= partialSolution[s - 1]
+  0 <= |solution| <= problem.numberOfObjects && 
+  forall k :: 0 <= k < |solution| ==> solution[k] == 0 || solution[k] == 1
 }
 
-predicate isOptimalSolution(p: Problem, solution: Solution)
-  requires isValidProblem(p)
-  requires isValidSolution(p, solution)  
+predicate isPartialSolution(problem: Problem, solution: seq<int>)
+  requires isValidProblem(problem)
 {
-    isSolution(p, solution) &&
-    forall s : Solution :: ((isSolution(p, s) && isValidSolution(p, s)) 
-    ==> gain(solution.objects, p.costs) >= gain(s.objects, p.costs))
+  isValidPartialSolution(problem, solution) && 
+  weight(problem, solution) < problem.knapsackCapacity
+}
+
+predicate isPartialSolutionOfProfitN(p: Problem, profits: seq<seq<int>>, x: int, y: int, n: int)
+{
+  0 <= x <= |profits| && (x > 0 ==> 0 <= y < |profits[x - 1]| && profits[x - 1][y] == n)
+  //  0 <= x <= |profits| && (x > 0 ==> 0 <= y < |profits[x - 1]| && exists a: int :: profits[x - 1][y] == a)
+}
+
+// predicate isCompleteSolutionOfProfitX()
+// {
+  
+// }
+
+ghost predicate isOptimalSolution(problem: Problem, solution: seq<int>)
+  requires isValidProblem(problem)
+  requires isValidSolution(problem, solution)  
+{
+    isSolution(problem, solution) &&
+    forall s: seq<int> :: (((isValidSolution(problem, s) && isSolution(problem, s)) ==> 
+    gain(problem, solution) >= gain(problem, s)))
 }
 
 method addSequence(existingSeq: seq<seq<int>>, newSeq: seq<int>, c: int) returns (result: seq<seq<int>>)
@@ -59,31 +104,37 @@ method addSequence(existingSeq: seq<seq<int>>, newSeq: seq<int>, c: int) returns
   result := existingSeq + [newSeq];
 }
 
-method getMaximProfit(p: Problem) returns (solution: Solution)
+method getMaximProfit(p: Problem) returns (solution: seq<int>)
   requires isValidProblem(p)
+  // ensures isValidSolution(p, solution)
   // ensures isSolution(p, solution)
 {
     var profits := []; 
     var maximProfit := 0;
-    var partialProfits := [];
     
+    var partSol := getKnapsackObjects(p, profits);
+    var N := intermediaryPartialSolution(partSol, p.gains); 
+
     var i := 0;
     while i <= p.numberOfObjects 
       invariant |profits| == i
       invariant 0 <= i <= p.numberOfObjects + 1
+      invariant |profits| <= p.numberOfObjects + 1
       invariant forall k :: 0 <= k < i ==> |profits[k]| == p.knapsackCapacity + 1
-      // invariant forall j :: 0 <= j < i ==> isPartialSolution(partialProfits)
+      invariant forall x :: 0 <= x < i ==> forall y :: 0 <= y <= p.knapsackCapacity ==> 
+        isPartialSolutionOfProfitN(p, profits, x, y, N)
     {
-        partialProfits := getPartialProfits(p, profits,i);
+        var partialProfits := getPartialProfits(p, profits, i);
         profits := addSequence(profits, partialProfits, p.knapsackCapacity + 1);
         i := i + 1;
+
+        partSol := getKnapsackObjects(p, profits);
+        N := intermediaryPartialSolution(partSol, p.gains); 
     }
 
     maximProfit := profits[p.numberOfObjects][p.knapsackCapacity];
 
-    var objects := getKnapsackObjects(p, profits, maximProfit);
-
-    solution := Solution(maximProfit, objects);
+    solution := getKnapsackObjects(p, profits);
 }
 
 method getPartialProfits(p: Problem, profits: seq<seq<int>>, i: int) returns (partialProfits: seq<int>)
@@ -92,67 +143,103 @@ method getPartialProfits(p: Problem, profits: seq<seq<int>>, i: int) returns (pa
   requires 0 <= i < p.numberOfObjects + 1
   requires forall k :: 0 <= k < i ==> |profits[k]| == p.knapsackCapacity + 1
   ensures |partialProfits| == p.knapsackCapacity + 1
-  // ensures isSolution(p, solution, maximProfit)
+  // ensures isSolution(p, solution)
 {
         partialProfits := [];
         var j := 0;
+
+        var partSol := getKnapsackObjects(p, profits);
+        var N := intermediaryPartialSolution(partSol, p.gains); 
+
         while j <= p.knapsackCapacity
           invariant 0 <= j <= p.knapsackCapacity + 1
           invariant |partialProfits| == j
-          // invariant isPartialSolution(partialProfits)
+          invariant forall y :: 0 <= y < j ==> isPartialSolutionOfProfitN(p, profits, i, y, N)
         {
           if i == 0 || j == 0 {
               partialProfits := partialProfits + [0];
           } else {
             if p.weights[i - 1] <= j {
-              partialProfits := partialProfits + [max(p.costs[i - 1] + profits[i - 1][j - p.weights[i - 1]], profits[i - 1][j])];
+              partialProfits := partialProfits + [max(p.gains[i - 1] + profits[i - 1][j - p.weights[i - 1]], profits[i - 1][j])];
             } else {
               partialProfits := partialProfits + [profits[i - 1][j]];
             }
           }
           j := j + 1;
+          partSol := getKnapsackObjects(p, profits);
+          N := intermediaryPartialSolution(partSol, p.gains); 
         }
 }
 
-method getKnapsackObjects(p: Problem, profits: seq<seq<int>>, maximProfit: int) returns (objectHasBeenAdded: seq<int>)
-  requires isValidProblem(p)
-  requires |profits| == p.numberOfObjects + 1
-  requires forall k :: 0 <= k <= p.numberOfObjects ==> |profits[k]| == p.knapsackCapacity + 1
-  // ensures isSolution(p, solution)
+// method getKnapsackObjects(p: Problem, profits: seq<seq<int>>) returns (solution: seq<int>)
+//   requires isValidProblem(p)
+//   requires |profits| == p.numberOfObjects + 1
+//   requires forall k :: 0 <= k <= p.numberOfObjects ==> |profits[k]| == p.knapsackCapacity + 1
+//   ensures isValidSolution(p, solution)
+// {
+//     solution := [];
+//     var i := p.numberOfObjects;
+//     var j := p.knapsackCapacity;
+
+//     while i > 0 && j >= 0
+//       invariant 0 <= i <= p.numberOfObjects
+//       invariant 0 <= j <= p.knapsackCapacity
+//       invariant |solution| == p.numberOfObjects - i
+//       invariant isPartialSolution(p, solution)
+//       decreases i
+//       decreases j
+//     {
+//       if profits[i][j] == profits[i - 1][j] {
+//         solution := [0] + solution;
+//         i := i - 1;
+//       } else { 
+//         solution := [1] + solution;
+//         i := i - 1;
+//         if j - p.weights[i] >= 0 {
+//           j := j - p.weights[i];
+//         }
+//       }
+//     }
+// }
+
+method getKnapsackObjects(p: Problem, profits: seq<seq<int>>) returns (solution: seq<int>)
+    requires isValidProblem(p)
+    requires forall k :: 0 <= k < |profits| ==> |profits[k]| == p.knapsackCapacity + 1
+    requires |profits| <= |p.weights| + 1
 {
-    objectHasBeenAdded := [];
-    var i := p.numberOfObjects;
+    solution := [];
+    var i := |profits| - 1;
     var j := p.knapsackCapacity;
 
     while i > 0 && j >= 0
-      invariant 0 <= i <= p.numberOfObjects
+      invariant -1 <= i <= |profits|
       invariant 0 <= j <= p.knapsackCapacity
-      invariant |objectHasBeenAdded| == p.numberOfObjects - i
+      invariant -1 <= i <= |p.weights|
+      invariant |solution| <= p.numberOfObjects - i
+      invariant isPartialSolution(p, solution)
       decreases i
       decreases j
     {
       if profits[i][j] == profits[i - 1][j] {
-        objectHasBeenAdded := [0] + objectHasBeenAdded;
+        solution := [0] + solution;
         i := i - 1;
       } else { 
-        objectHasBeenAdded := [1] + objectHasBeenAdded;
+        solution := [1] + solution;
         i := i - 1;
         if j - p.weights[i] >= 0 {
           j := j - p.weights[i];
         }
-        
       }
     }
-    // assert |objectHasBeenAdded| == |p.weights|;
 }
 
 method Main()
 {
     var problem: Problem := Problem(numberOfObjects := 4, knapsackCapacity := 8, 
-                                    costs := [1, 2, 5, 6], weights := [2, 3, 4, 5]);
+                                    gains := [1, 2, 5, 6], weights := [2, 3, 4, 5]);
     var solution := getMaximProfit(problem);
 
     print "Maxim profit: ";
-    print solution.profit;
+    // print gain(problem, solution);
     print "\n";
 }
